Added the design Hoare logic, and some additional design laws. Changed memory programs and separation logic so it uses this instead, and we can therefore prove the auxiliary frame rule via the locality property (as formalised in Dongol, Gomes, and Struth 2015).

theories/memory/utp_seplog.thy
@@ -4,6 +4,8 @@ theory utp_seplog
   imports utp_memory
 begin
 
+subsection \<open> Operators \<close>
+
 type_synonym 's spred = "'s mem upred"
 
 definition empty_heap :: "'s spred" ("emp") where [upred_defs]: "emp = (dom\<^sub>u(&hp) =\<^sub>u {}\<^sub>u)"
@@ -25,49 +27,102 @@ abbreviation heaplet_min :: "(addr, 's) uexpr \<Rightarrow> ('a::countable, 's) 
 abbreviation heaplet_ex :: "(addr, 's) uexpr \<Rightarrow> 's spred" ("_ \<^bold>\<mapsto> -" [69] 70) where
 "e \<^bold>\<mapsto> - \<equiv> (\<^bold>\<exists> v::nat \<bullet> e \<^bold>\<mapsto> \<guillemotleft>v\<guillemotright>)"
 
+subsection \<open> Algebraic Properties \<close>
+
 lemma sep_conj_comm: "(P \<^bold>* Q) = (Q \<^bold>* P)"
   using ffun_plus_commute by (rel_blast)
 
 lemma sep_conj_assoc: "((P \<^bold>* Q) \<^bold>* R) = (P \<^bold>* (Q \<^bold>* R))"
-  apply (rel_auto) oops
+  apply (rel_auto)
+   apply (rename_tac st h0 h1 h2)
+   apply (rule_tac x="h1" in exI)
+   apply (rule_tac x="h0 + h2" in exI)
+  apply (auto simp add: Int_Un_distrib2 add.assoc ffun_plus_commute)
+   apply (rename_tac st h0 h1 h2)
+  apply (rule_tac x="h0 + h1" in exI)
+  apply (rule_tac x="h2" in exI)
+  apply (auto simp add: Int_Un_distrib2 add.assoc ffun_plus_commute)
+  done
+
+lemma sep_conj_iso: "P \<sqsubseteq> Q \<Longrightarrow> (P \<^bold>* R) \<sqsubseteq> (Q \<^bold>* R)"
+  by (rel_auto)
 
 lemma sep_conj_unit: "(emp \<^bold>* P) = P"
   apply (rel_auto)
   apply (metis add.left_neutral bounded_semilattice_sup_bot_class.sup_bot.left_neutral ffun_minus_plus_commute ffun_minus_self ffun_minus_zero lattice_class.inf_sup_absorb)
   using fdom_zero by fastforce
 
+subsection \<open> Locality \<close>
+
+definition local_wrt :: "'s spred \<Rightarrow> 's sprog \<Rightarrow> bool" where
+[upred_defs]: "local_wrt p S = (\<forall> q. (S wp\<^sub>D (p \<^bold>* q) \<sqsubseteq> (p \<^bold>* (S wp\<^sub>D q))))"
+
+lemma local_wrt_seq_closed:
+  assumes "C is \<^bold>N" "D is \<^bold>N" "local_wrt r C" "local_wrt r D"
+  shows "local_wrt r (C ;; D)"
+proof -
+  obtain c\<^sub>1 C\<^sub>2 where C: "C = c\<^sub>1 \<turnstile>\<^sub>n C\<^sub>2"
+    by (metis assms(1) ndesign_form)
+  obtain d\<^sub>1 D\<^sub>2 where D: "D = d\<^sub>1 \<turnstile>\<^sub>n D\<^sub>2"
+    by (metis assms(2) ndesign_form)
+  with assms(3-4) show ?thesis
+    apply (simp add: C D local_wrt_def wp)
+    apply (auto)
+    apply (metis wp_conj)
+    apply (metis utp_pred_laws.inf.absorb_iff2 utp_pred_laws.le_infE wp_conj)
+    apply (metis utp_pred_laws.inf.absorb_iff2 utp_pred_laws.inf_assoc wp_conj)
+    done
+qed
+
+lemma local_wrt_heap_lookup: 
+  "\<lbrakk> vwb_lens x; x \<sharp> e; st:x \<sharp> p \<rbrakk> \<Longrightarrow> local_wrt p (x := *e)"
+  apply (rel_simp)
+  apply (rename_tac q st hp0 hp1)
+  apply (rule_tac x="hp0" in exI)
+  apply (auto)
+  done
+
+subsection \<open> Separation Logic Laws \<close>
+
+lemma frame_rule_aux:
+  "\<lbrakk> c is \<^bold>N; local_wrt r c; {p} c {q}\<^sub>D \<rbrakk> \<Longrightarrow> {p \<^bold>* r} c {q \<^bold>* r}\<^sub>D"
+  apply (simp add: wp_hoare_d_link)
+  apply (simp add: local_wrt_def)
+  apply (metis (no_types, lifting) dual_order.trans sep_conj_comm sep_conj_iso)
+  done
+
 lemma allocation_noninterfering_local:
-  "\<lbrace>emp\<rbrace>v := alloc(e)\<lbrace>&v \<^bold>\<mapsto> e\<rbrace>\<^sub>u"
+  "{emp}v := alloc(e){&v \<^bold>\<mapsto> e}\<^sub>D"
   by (rel_auto)
 
 lemma allocation_noninterfering_global:
-  "\<lbrakk> vwb_lens x; st:x \<sharp> p \<rbrakk> \<Longrightarrow> \<lbrace>p\<rbrace>x := alloc(e)\<lbrace>p \<^bold>* &x \<^bold>\<mapsto> e\<rbrace>\<^sub>u"
+  "\<lbrakk> vwb_lens x; st:x \<sharp> p \<rbrakk> \<Longrightarrow> {p}x := alloc(e){p \<^bold>* &x \<^bold>\<mapsto> e}\<^sub>D"
   apply (rel_simp)
-  apply (rename_tac st hp l)
+  apply (rename_tac ok st hp ok' l)
   apply (rule_tac x="hp" in exI)
   apply (rule_tac x="0(l \<mapsto> to_nat (\<lbrakk>e\<rbrakk>\<^sub>e (put\<^bsub>x\<^esub> st l)))\<^sub>f" in exI)
   apply (auto)
   done
 
-lemma mutation_local: "\<lbrace>e \<^bold>\<mapsto> -\<rbrace> *e := v \<lbrace>e \<^bold>\<mapsto> v\<rbrace>\<^sub>u"
+lemma mutation_local: "{e \<^bold>\<mapsto> -} *e := v {e \<^bold>\<mapsto> v}\<^sub>D"
   by (rel_auto)
 
-lemma mutation_global: "\<lbrace>p \<^bold>* e \<^bold>\<mapsto> -\<rbrace> *e := v \<lbrace>p \<^bold>* e \<^bold>\<mapsto> v\<rbrace>\<^sub>u"
+lemma mutation_global: "{p \<^bold>* e \<^bold>\<mapsto> -} *e := v {p \<^bold>* e \<^bold>\<mapsto> v}\<^sub>D"
   apply (rel_simp)
-  apply (rename_tac st a b x)
+  apply (rename_tac st ok' a b x)
   apply (rule_tac x="a" in exI)
   apply (rule_tac x="b(\<lbrakk>e\<rbrakk>\<^sub>e st \<mapsto> to_nat (\<lbrakk>v\<rbrakk>\<^sub>e st))\<^sub>f" in exI)
   apply (simp)
   done
 
 lemma deallocation_local:
-  "\<lbrace>e \<^bold>\<mapsto> -\<rbrace> dealloc(e) \<lbrace>emp\<rbrace>\<^sub>u"
+  "{e \<^bold>\<mapsto> -} dealloc(e) {emp}\<^sub>D"
   by (rel_auto)
 
 lemma deallocation_global:
-  "\<lbrace>r \<^bold>* e \<^bold>\<mapsto> -\<rbrace> dealloc(e) \<lbrace>r\<rbrace>\<^sub>u"
+  "{r \<^bold>* e \<^bold>\<mapsto> -} dealloc(e) {r}\<^sub>D"
   apply (rel_simp)
-  apply (rename_tac st a b x)
+  apply (rename_tac ok st ok' a b x)
   apply (subgoal_tac "fdom(a) \<lhd>\<^sub>f b = fdom(a) \<lhd>\<^sub>f (fdom(b) \<lhd>\<^sub>f b)")
    apply (simp)
   apply (fastforce)
@@ -75,23 +130,7 @@ lemma deallocation_global:
 
 lemma lookup_global:
   "\<lbrakk> vwb_lens x; x \<sharp> e; x \<sharp> v; st:x \<sharp> r \<rbrakk> \<Longrightarrow> 
-    \<lbrace>r \<^bold>* e \<^bold>\<mapsto> v\<rbrace> x := *e \<lbrace>r \<^bold>* (&st:x =\<^sub>u (v \<oplus>\<^sub>p st) \<and> e \<^bold>\<mapsto> v)\<rbrace>\<^sub>u"
+    {r \<^bold>* e \<^bold>\<mapsto> v} x := *e {r \<^bold>* (&st:x =\<^sub>u (v \<oplus>\<^sub>p st) \<and> e \<^bold>\<mapsto> v)}\<^sub>D"
   by (rel_simp, metis (full_types) Diff_Diff_Int Diff_insert0 Int_empty_right)
   
-lemma frame_rule:
-  "vwb_lens x \<Longrightarrow> \<lbrace>p\<rbrace> c \<lbrace>q\<rbrace>\<^sub>u \<Longrightarrow> \<lbrace>p \<^bold>* r\<rbrace> c \<lbrace>q \<^bold>* r\<rbrace>\<^sub>u"
-  apply (rel_simp)
-  oops
-
-text \<open> Safety Monotonicity \<close>
-
-definition safety_mono :: "'s sprog \<Rightarrow> bool" where
-[upred_defs]: "safety_mono P = (\<forall> s\<^sub>0 s\<^sub>1. \<lbrakk>Dom(P)\<rbrakk>\<^sub>e s\<^sub>0 \<and> s\<^sub>0 \<le> s\<^sub>1 \<longrightarrow> \<lbrakk>Dom(P)\<rbrakk>\<^sub>e s\<^sub>1)"
-
-lemma safety_mono_dealloc: "safety_mono (dealloc(e))"
-  by (rel_simp, meson contra_subsetD fsubseteq_dom_subset)
-
-lemma safety_mono_choice: "\<lbrakk> safety_mono P; safety_mono Q \<rbrakk> \<Longrightarrow> safety_mono (P \<sqinter> Q)"
-  by (rel_blast)
-
 end
