theories/memory/utp_memory.thy
@@ -1,7 +1,7 @@
 section \<open> Programs with memory \<close>
 
 theory utp_memory
-  imports "UTP.utp"
+  imports "UTP-Designs.utp_designs"
 begin
 
 text \<open> For now we represent addresses and data as naturals. We can therefore inject
@@ -31,15 +31,15 @@ begin
   instance by (intro_classes, (rel_auto)+)
 end
 
-text \<open> A program is simply a homogeneous relation with a memory state space. \<close>
+text \<open> A program is simply a homogeneous design with a memory state space. \<close>
 
-type_synonym 's sprog = "'s mem hrel"
+type_synonym 's sprog = "'s mem hrel_des"
 
 text \<open> An abort is currently just the empty relation. In future we could use the theory
   of designs instead and model aborts differently. \<close>
 
 abbreviation abort_mp :: "'s sprog" ("abort") where
-"abort \<equiv> false"
+"abort \<equiv> true"
 
 text \<open> Heap allocation takes a lens $x$ within the store that holds an address, and an expression
   $e$ over store variables whose return type is countable. The semantics of allocation selects
@@ -49,35 +49,50 @@ text \<open> Heap allocation takes a lens $x$ within the store that holds an add
 definition
   heap_alloc :: "(addr \<Longrightarrow> 's) \<Rightarrow> ('a::countable, 's) uexpr \<Rightarrow> 's sprog"
   ("_ := alloc'(_')" [74,0] 75) 
-  where [upred_defs]: 
+  where [upred_defs, ndes_simp]: 
     "x := alloc(e) = 
-     (\<Sqinter> l | \<guillemotleft>l\<guillemotright> \<notin>\<^sub>u dom\<^sub>u($hp) \<bullet> st:x := \<guillemotleft>l\<guillemotright> ;; hp := &hp(&st:x \<mapsto> uop to_nat (e \<oplus>\<^sub>p st))\<^sub>u)"
+     (true \<turnstile>\<^sub>n (\<Sqinter> l | \<guillemotleft>l\<guillemotright> \<notin>\<^sub>u dom\<^sub>u($hp) \<bullet> st:x := \<guillemotleft>l\<guillemotright> ;; hp := &hp(&st:x \<mapsto> uop to_nat (e \<oplus>\<^sub>p st))\<^sub>u))"
 
 text \<open> Heap lookup retrieves data from the heap and places it into a store variable. If the memory
   location $l$ is unallocated then an abort is the result. \<close>
 
 definition 
-  heap_lookup :: "('a::countable \<Longrightarrow> 's) \<Rightarrow> (addr, 's) uexpr \<Rightarrow> 's mem hrel" 
+  heap_lookup :: "('a::countable \<Longrightarrow> 's) \<Rightarrow> (addr, 's) uexpr \<Rightarrow> 's sprog" 
   ("_ := *_" [74,75] 75)
-  where [upred_defs]: 
-    "x := *l = (\<lceil>(l \<oplus>\<^sub>p st) \<in>\<^sub>u dom\<^sub>u(&hp)\<rceil>\<^sub>< \<and> st:x := uop from_nat (&hp(l \<oplus>\<^sub>p st)\<^sub>a))"
+  where [upred_defs, ndes_simp]: 
+    "x := *l = (((l \<oplus>\<^sub>p st) \<in>\<^sub>u dom\<^sub>u(&hp)) \<turnstile>\<^sub>n st:x := uop from_nat (&hp(l \<oplus>\<^sub>p st)\<^sub>a))"
 
 text \<open> Heap mutation updates the value of an already allocated address in the heap. \<close>
 
 definition
-  heap_mutate :: "(addr, 's) uexpr \<Rightarrow> ('a::countable, 's) uexpr \<Rightarrow> 's mem hrel"
+  heap_mutate :: "(addr, 's) uexpr \<Rightarrow> ('a::countable, 's) uexpr \<Rightarrow> 's sprog"
   ("*_ := _" [0, 74] 75)
-  where [upred_defs]:
-    "*l := e = (\<lceil>(l \<oplus>\<^sub>p st) \<in>\<^sub>u dom\<^sub>u(&hp)\<rceil>\<^sub>< \<and> hp := &hp((l \<oplus>\<^sub>p st) \<mapsto> uop to_nat (e \<oplus>\<^sub>p st))\<^sub>u)"
+  where [upred_defs, ndes_simp]:
+    "*l := e = (((l \<oplus>\<^sub>p st) \<in>\<^sub>u dom\<^sub>u(&hp)) \<turnstile>\<^sub>n hp := &hp((l \<oplus>\<^sub>p st) \<mapsto> uop to_nat (e \<oplus>\<^sub>p st))\<^sub>u)"
 
 text \<open> Heap deallocation removes an area of memory from the heap. \<close>
 
 definition
-  heap_dealloc :: "(addr, 's) uexpr \<Rightarrow> 's mem hrel" ("dealloc'(_')")
-  where [upred_defs]:
-  "dealloc(l) = (\<lceil>(l \<oplus>\<^sub>p st) \<in>\<^sub>u dom\<^sub>u(&hp)\<rceil>\<^sub>< \<and> hp := (dom\<^sub>u(&hp) - {l \<oplus>\<^sub>p st}\<^sub>u) \<lhd>\<^sub>u &hp)"
+  heap_dealloc :: "(addr, 's) uexpr \<Rightarrow> 's sprog" ("dealloc'(_')")
+  where [upred_defs, ndes_simp]:
+  "dealloc(l) = (((l \<oplus>\<^sub>p st) \<in>\<^sub>u dom\<^sub>u(&hp)) \<turnstile>\<^sub>n hp := (dom\<^sub>u(&hp) - {l \<oplus>\<^sub>p st}\<^sub>u) \<lhd>\<^sub>u &hp)"
 
-text \<open> Some example properties \<close>
+subsection \<open> Weakest Precondition Semantics \<close>
+
+lemma wp_UINF_pred [wp]:
+  "\<lbrakk> \<And> l. out\<alpha> \<sharp> P(l) \<rbrakk> \<Longrightarrow> (\<Sqinter> l | P(l) \<bullet> Q(l)) wp q = (\<^bold>\<forall> l \<bullet> \<lfloor>P(l)\<rfloor>\<^sub>< \<Rightarrow> (Q(l) wp q))"
+  by (rel_blast)
+
+lemma wp_heap_alloc [wp]:
+  "\<lbrakk> vwb_lens x; x \<sharp> e \<rbrakk> \<Longrightarrow> 
+   x := alloc(e) wp\<^sub>D p = (\<^bold>\<forall> l \<in> -dom\<^sub>u(&hp) \<bullet> p\<lbrakk>\<guillemotleft>l\<guillemotright>,&hp(\<guillemotleft>l\<guillemotright> \<mapsto> uop to_nat (e \<oplus>\<^sub>p st))\<^sub>u/&st:x,&hp\<rbrakk>)"
+  by (simp add: ndes_simp wp usubst unrest, rel_auto)
+
+lemma wp_heap_dealloc [wp]: 
+  "dealloc(e) wp\<^sub>D p = (e \<oplus>\<^sub>p st \<in>\<^sub>u dom\<^sub>u(&hp) \<and> p\<lbrakk>(dom\<^sub>u(&hp) - {e \<oplus>\<^sub>p st}\<^sub>u) \<lhd>\<^sub>u &hp/&hp\<rbrakk>)"
+  by (rel_auto)
+
+subsection \<open> Example properties \<close>
 
 lemma least_nat_Compl_not_in [simp]:
   fixes A :: "nat set"
@@ -85,18 +100,18 @@ lemma least_nat_Compl_not_in [simp]:
   shows "Inf(- A) \<notin> A"
   by (metis ComplD ComplI Inf_nat_def assms ex_new_if_finite infinite_UNIV wellorder_Least_lemma(1))
 
-lemma "(x := alloc(\<guillemotleft>u\<guillemotright>) ;; *&x := \<guillemotleft>v\<guillemotright>) = (x := alloc(\<guillemotleft>v\<guillemotright>))"
-  by (rel_auto)
+lemma "(x := alloc(\<guillemotleft>u\<guillemotright>) ;; *&x := \<guillemotleft>v\<guillemotright>) = (x := alloc(\<guillemotleft>v\<guillemotright>))"  
+  by (rel_auto, fastforce)
 
 lemma "dealloc(e) ;; dealloc(e) = abort"
-  by (rel_auto)
+  by (ndes_simp, rel_auto)
 
 lemma "dealloc(e) ;; *e := \<guillemotleft>v\<guillemotright> = abort"
-  by (rel_auto)
+  by (ndes_simp, rel_auto)
 
-lemma "vwb_lens x \<Longrightarrow> (x := alloc(\<guillemotleft>5 :: int\<guillemotright>) ;; dealloc(&x) ;; st:x := 0) = st:x := 0"
-  apply (rel_auto)
-  apply (rename_tac st hp)
+lemma "vwb_lens x \<Longrightarrow> (x := alloc(\<guillemotleft>5 :: int\<guillemotright>) ;; dealloc(&x) ;; st:x :=\<^sub>D 0) = st:x :=\<^sub>D 0"
+  apply (ndes_simp, rel_auto)
+  apply (rename_tac ok st hp ok')
   apply (rule_tac x="put\<^bsub>x\<^esub> st (\<Squnion>(- fdom(hp)))" in exI, simp)
   apply (rule_tac x="hp(Inf(- fdom(hp)) \<mapsto> to_nat 5)\<^sub>f" in exI)
   apply (auto)
